Precisely track capacity for memLog
Needed to append to it, and unfortunately our support for slice capacity
is not great. It would have been nice to have better predicates for
talking about subslices precisely without involving the model of slices
or u64s everywhere, but capacity is just hard to correctly fit into the
reasoning regardless.

src/goose_lang/lib/slice/slice.v
@@ -40,15 +40,23 @@ doesn't make use of capacity *)
 Definition is_slice_small (s: Slice.t) (t:ty) (q:Qp) (vs: list val): iProp Σ :=
   s.(Slice.ptr) ↦∗[t]{q} vs ∗ ⌜length vs = int.nat s.(Slice.sz)⌝.
 
-Definition is_slice (s: Slice.t) (t:ty) (q:Qp) (vs: list val): iProp Σ :=
-  is_slice_small s t q vs ∗
+Definition is_slice_cap (s: Slice.t) (t:ty): iProp Σ :=
   (∃ extra, ⌜Z.of_nat (length extra) = Slice.extra s⌝ ∗
             (s.(Slice.ptr) +ₗ[t] int.val s.(Slice.sz)) ↦∗[t] extra).
+
+Definition is_slice (s: Slice.t) (t:ty) (q:Qp) (vs: list val): iProp Σ :=
+  is_slice_small s t q vs ∗ is_slice_cap s t.
 
 Lemma is_slice_to_small s t q vs :
   is_slice s t q vs -∗ is_slice_small s t q vs.
 Proof.
   iDestruct 1 as "[$ _]".
+Qed.
+
+Lemma is_slice_split s t q vs :
+  is_slice s t q vs ⊣⊢ is_slice_small s t q vs ∗ is_slice_cap s t.
+Proof.
+  rewrite /is_slice //.
 Qed.
 
 Lemma is_slice_small_acc s t q vs :
@@ -298,7 +306,9 @@ Proof.
   iSplitR.
   { iPureIntro.
     rewrite replicate_length.
+    simpl.
     word. }
+  simpl.
   iExactEq "Hextra"; word_eq.
 Qed.
 
@@ -808,6 +818,7 @@ Proof.
       iPureIntro.
       word. }
     iExists extra'.
+    simpl.
     iSplitR; first by iPureIntro; word.
     rewrite loc_add_assoc.
     iExactEq "Hfree"; word_eq.
@@ -853,7 +864,9 @@ Proof.
       iSplitR.
       { rewrite replicate_length.
         iPureIntro.
+        simpl.
         word. }
+      simpl.
       iExactEq "HnewFree"; word_eq.
 Qed.
 
